support for null pointer

ulib/experimental/Steel.C.Reference.fst
@@ -1,20 +1,31 @@
 module Steel.C.Reference
-open FStar.FunctionalExtensionality
 open Steel.C.PCM
-open Steel.C.Connection
 open Steel.C.Ref
 open Steel.Effect
 open Steel.Effect.Atomic
 
-open FStar.FSet
-
 #push-options "--print_universes"
 
-let ref (a: Type u#0) (view_t: Type u#0) (#b: Type u#b) (q: pcm b)
+// [@@__reduce__]
+let ptr (a: Type u#0) (view_t: Type u#0) (#b: Type u#b) (q: pcm b)
 : Type u#b
-= ref a q
+= ptr a q
 
-[@@__steel_reduce__]
+// [@@__reduce__]
+inline_for_extraction
+let ref (a: Type u#0) (view_t: Type u#0) (#b: Type u#b) (q: pcm b)
+: Tot (Type u#b)
+=
+  (x: ptr a view_t q { not_null x })
+
+unfold
+let ref_of_ref
+  (#a: Type u#0) (#view_t: Type u#0) (#b: Type u#b) (#q: pcm b)
+  (r: ref a view_t q)
+: Tot (Steel.C.Ref.ref a q)
+= r
+
+[@@__steel_reduce__] // ; __reduce__]
 let pts_to_view
   (#a: Type u#0) 
   (#view_t: Type u#0)
@@ -24,19 +35,10 @@ let pts_to_view
 : vprop
 = r `pts_to_view` view
 
-(*
-val ref_alloc
-  (#a:Type0) (p: pcm a) (x: a)
-: Steel (ref a p)
-    emp
-    (fun r -> r `pts_to` x)
-    (requires fun _ -> p_refine p x)
-    (ensures fun _ _ _ -> True)
-*)
-
 let ref_read
-  (#a: Type u#0) (#b: Type u#b) (#p: pcm b)
+  (#a: Type u#0) (#b: Type u#b)
   (#view_t: Type u#0)
+  (#p: pcm b)
   (#vw: sel_view p view_t false)
   (r: ref a view_t p)
 : Steel view_t
@@ -48,3 +50,85 @@ let ref_read
     res == h' (r `pts_to_view` vw)
   ))
 = ref_read_sel r vw
+
+let null (a: Type u#0) (view_t: Type u#0) (#b: Type u#b) (p: pcm b) : Tot (ptr a view_t p) = null a p
+
+[@@__steel_reduce__] // ; __reduce__]
+let pts_to_view_or_null
+  (#a: Type u#0) 
+  (#view_t: Type u#0)
+  (#view_t': Type u#0)
+  (#b: Type u#b) (#p: pcm b)
+  (r: ptr a view_t p) (view: sel_view p view_t' false)
+: vprop
+= r `pts_to_view_or_null` view
+
+let is_null
+  (#a: Type u#0) (#b: Type u#b) (#c: Type0) (#p: pcm b)
+  (r: ptr a c p)
+  (vw: sel_view p c false)
+: Steel bool
+    (pts_to_view_or_null r vw)
+    (fun _ -> pts_to_view_or_null r vw)
+    (requires (fun _ -> True))
+    (ensures (fun h res h' ->
+      let s = h (pts_to_view_or_null r vw) in
+      h' (pts_to_view_or_null r vw) == s /\
+      res == ptr_is_null r /\
+      res == (None? s)
+    ))
+= is_null r vw
+
+let intro_pts_to_view_or_null_null
+  (#inames: _)
+  (a: Type) (#b: Type) (#p: pcm b)
+  (#c: Type0)
+  (vw: sel_view p c false)
+: SteelGhost unit inames
+    emp
+    (fun _ -> pts_to_view_or_null (null a c p) vw)
+    (requires (fun _ -> True))
+    (ensures (fun _ _ h' -> h' (pts_to_view_or_null (null a c p) vw) == None))
+= intro_pts_to_view_or_null_null a vw
+
+let elim_pts_to_view_or_null_null
+  (#inames: _)
+  (a: Type) (#b: Type) (#p: pcm b)
+  (#c: Type0)
+  (vw: sel_view p c false)
+: SteelGhostT unit inames
+    (pts_to_view_or_null (null a c p) vw)
+    (fun _ -> emp)
+= elim_pts_to_view_or_null_null a vw
+
+let intro_pts_to_view_or_null_not_null
+  (#inames: _)
+  (#a: Type) (#b: Type) (#p: pcm b)
+  (#c: Type0)
+  (r: ref a c p)
+  (vw: sel_view p c false)
+: SteelGhost unit inames
+    (pts_to_view r vw)
+    (fun _ -> pts_to_view_or_null r vw)
+    (requires (fun _ -> True))
+    (ensures (fun h _ h' -> h' (pts_to_view_or_null r vw) == Some (h (pts_to_view r vw))))
+= intro_pts_to_view_or_null_not_null r vw
+
+let elim_pts_to_view_or_null_not_null
+  (#inames: _)
+  (#a: Type) (#b: Type) (#p: pcm b)
+  (#c: Type0)
+  (r: ref a c p)
+  (vw: sel_view p c false)
+: SteelGhost unit inames
+    (pts_to_view_or_null r vw)
+    (fun _ -> pts_to_view r vw)
+    (requires (fun _ -> True))
+    (ensures (fun h _ h' -> h (pts_to_view_or_null r vw) == Some (h' (pts_to_view r vw))))
+= elim_pts_to_view_or_null_not_null r vw
+
+let freeable
+  (#a: Type u#0) (#view_t: Type u#0) (#b: Type u#0) (#q: pcm b)
+  (r: ref a view_t q)
+: Tot prop
+= freeable (r <: Steel.C.Ref.ref a q)
